ESPL: Make wildcards explicit

data/isabelle/src/ESPLogic/ExplicitModel.thy
@@ -111,12 +111,10 @@ lemma longTermKeys_conv:
 
 type_synonym state = "explicit_trace \<times> threadpool \<times> store"
 
-definition not_match_concl :: "role \<Rightarrow> store => tid \<Rightarrow> rolestep \<Rightarrow> bool"
-where
-  "not_match_concl R s i step = all_args (var_map (\<lambda>rhs. Some (s (matchVar step, i)) \<noteq> rhs)
-                                          (inst_free (wildcards R step) s i (stepPat step)))"
 
-declare not_match_concl_def[simp]
+definition exec_match :: "store \<Rightarrow> tid \<Rightarrow> varid \<Rightarrow> pattern \<Rightarrow> bool"
+where
+  "exec_match s i v pt = var_fold Ex (var_map (op = (Some (s (v, i)))) (any_inst s i pt))"
 
 inductive_set 
   reachable :: "proto \<Rightarrow> state set" 
@@ -158,9 +156,7 @@ where
 
 | match: "\<lbrakk> (t, r, s) \<in> reachable P;
             r i = Some (done, Match l eq mv pt # todo, skipped);
-            if eq
-              then Some (s (mv, i)) = inst s i pt
-              else not_match_concl (done @ Match l eq mv pt # todo) s i (Match l eq mv pt)
+            exec_match s i mv pt = eq
           \<rbrakk>
           \<Longrightarrow> (t @ [Step (i, Match l eq mv pt)], r(i \<mapsto> (done @ [Match l eq mv pt], todo, skipped)), s) \<in> reachable P"
 
@@ -1202,75 +1198,20 @@ lemma Ln_before_inpE:
    \<rbrakk> \<Longrightarrow> Q"
   by (auto dest!: Ln_before_inp)
 
-lemma Match_eq:
-  "(i, Match l True v pt) \<in> steps t \<Longrightarrow> Some (s (v, i)) = inst s i pt"
-by (induct rule: reachable_induct) (fastforce+)
-
-lemma Not_Match:
-  "\<lbrakk> r i = Some (done, todo, skipped);
-     (i, Match l False v pt) \<in> steps t
-   \<rbrakk> \<Longrightarrow> not_match_concl (done @ todo) s i (Match l False v pt)"
-proof (induct arbitrary: "done" todo skipped rule: reachable_induct)
-  let ?step = "Match l False v pt"
-  case (match t r s i' done' l' eq' v' pt' todo' skipped')
-    let ?step' = "Match l' eq' v' pt'"
-    show ?case proof (cases "i = i'")
-      case True
-      note same_thread = this
-      hence steps: "done = done' @ [?step']" "todo = todo'" using match by auto
-      show ?thesis proof (cases "(i, ?step) \<in> steps t")
-        case True
-        hence "not_match_concl (done' @ ?step' # todo') s i ?step"
-          using same_thread match by blast
-        thus ?thesis using steps by simp
-      next
-        case False
-        hence "?step = ?step'" using match by auto
-        moreover hence "not_match_concl (done' @ ?step' # todo') s i ?step'"
-          using same_thread match by auto
-        ultimately show ?thesis using steps by simp
-      qed
-    qed (insert match, auto)
-next
-  case (compr t r s i' done' l ty pt todo' skipped')
-  let ?step = "Note l ty pt"
-  show ?case proof (cases "i = i'")
-    case True
-    moreover hence "done = done' @ [?step]" "todo = todo'" using compr by auto
-    ultimately show ?thesis using compr by fastforce
-  qed (insert compr, auto)
-next
-  case (skip t r s i' done' l ty pt todo' skipped')
-  let ?step = "Note l ty pt"
-  show ?case proof (cases "i = i'")
-    case True
-    moreover hence "done = done' @ [?step]" "todo = todo'" using skip by auto
-    ultimately show ?thesis using skip by fastforce
-  qed (insert skip, auto)
-next
-  case (send t r s i' done' l pt todo' skipped')
-  let ?step = "Send l pt"
-  show ?case proof (cases "i = i'")
-    case True
-    moreover hence "done = done' @ [?step]" "todo = todo'" using send by auto
-    ultimately show ?thesis using send by fastforce
-  qed (insert send, auto)
-next
-  case (recv t r s i' done' l pt todo' skipped')
-  let ?step = "Recv l pt"
-  show ?case proof (cases "i = i'")
-    case True
-    moreover hence "done = done' @ [?step]" "todo = todo'" using recv by auto
-    ultimately show ?thesis using recv by fastforce
-  qed (insert recv, auto)
-qed auto
-
 (*
 lemmas knows_inp = in_knows_predOrd1[OF Ln_before_inp, rule_format]
 *)
 
 text{* Three of the lemmas for the reasoning technique. *}
 lemmas Input = Ln_before_inp
+
+lemma match_eq_rule:
+  "(i, Match l True v pt) \<in> steps t \<Longrightarrow> exec_match s i v pt"
+by (induct rule: reachable_induct) (fastforce+)
+
+lemma not_match_rule:
+  "(i, Match l False v pt) \<in> steps t \<Longrightarrow> \<not> exec_match s i v pt"
+by (induct rule: reachable_induct) (fastforce+)
 
 lemma split_before:
   "Ln (Tup m m') \<prec> y \<Longrightarrow> Ln m \<prec> y \<and> Ln m' \<prec> y"
